1. Make check_precondition slightly more lenient. 2. Improve/simplify verif_object specification.

progs/verif_object.v
@@ -7,42 +7,40 @@ Definition Vprog : varspecs. mk_varspecs prog. Defined.
 Local Open Scope Z.
 Local Open Scope logic.
 
-Record object_schema : Type :=
- build_object_schema {
-   object_type: type;
-   object_invariant: list Z -> val -> mpred;
-}.
+Definition object_invariant := list Z -> val -> mpred.
 
 Definition tobject := tptr (Tstruct _object noattr).
 
-Definition reset_spec (schema: object_schema) :=
+Definition reset_spec (instance: object_invariant) :=
   WITH self: val, history: list Z
   PRE [ _self OF tobject]
           PROP ()
           LOCAL (temp _self self)
-          SEP (object_invariant schema history self)
+          SEP (instance history self)
   POST [ tvoid ]
-          PROP() LOCAL () SEP(object_invariant schema nil self).
+          PROP() LOCAL () SEP(instance nil self).
 
-Definition twiddle_spec (schema: object_schema) :=
+Definition twiddle_spec (instance: object_invariant) :=
   WITH self: val, i: Z, history: list Z
   PRE [ _self OF tobject, _i OF tint]
-          PROP ()
+          PROP (0 < i)
           LOCAL (temp _self self; temp _i (Vint (Int.repr i)))
-          SEP (object_invariant schema history self)
+          SEP (instance history self)
   POST [ tint ]
-          PROP() LOCAL (temp ret_temp (Vint (Int.repr (i + 2 * fold_right Z.add 0 history)))) 
-          SEP(object_invariant schema (i::history) self).
+      EX v: Z, 
+          PROP(2* fold_right Z.add 0 history < v <= 2* fold_right Z.add 0 (i::history))
+          LOCAL (temp ret_temp (Vint (Int.repr v))) 
+          SEP(instance (i::history) self).
 
-Definition object_methods (schema: object_schema) (mtable: val) : mpred :=
+Definition object_methods (instance: object_invariant) (mtable: val) : mpred :=
   EX sh: share, EX reset: val, EX twiddle: val,
   !! readable_share sh && 
-  func_ptr' (reset_spec schema) reset *
-  func_ptr' (twiddle_spec schema) twiddle *
+  func_ptr' (reset_spec instance) reset *
+  func_ptr' (twiddle_spec instance) twiddle *
   data_at sh (Tstruct _methods noattr) (reset,twiddle) mtable.
 
-Lemma object_methods_local_facts: forall schema p,
-  object_methods schema p |-- !! isptr p.
+Lemma object_methods_local_facts: forall instance p,
+  object_methods instance p |-- !! isptr p.
 Proof.
 intros.
 unfold object_methods.
@@ -52,32 +50,31 @@ Qed.
 Hint Resolve object_methods_local_facts : saturate_local.
 
 Definition object_mpred (history: list Z) (self: val) : mpred :=
-  EX schema: object_schema, EX mtable: val, 
-       (object_methods schema mtable *
+  EX instance: object_invariant, EX mtable: val, 
+       (object_methods instance mtable *
      field_at Tsh (Tstruct _object noattr) [StructField _mtable] mtable self*
-     object_invariant schema history self).
+     instance history self).
 
-Definition foo_schema : object_schema :=
-  build_object_schema (Tstruct _foo_object noattr)
+Definition foo_invariant : object_invariant :=
   (fun (history: list Z) p => field_at Tsh (Tstruct _foo_object noattr) 
             [StructField _data] (Vint (Int.repr (2*fold_right Z.add 0 history))) p
       *  malloc_token Tsh (sizeof (Tstruct _foo_object noattr)) p).
 
 Definition foo_reset_spec :=
- DECLARE _foo_reset (reset_spec foo_schema).
+ DECLARE _foo_reset (reset_spec foo_invariant).
 
 Definition foo_twiddle_spec :=
- DECLARE _foo_twiddle  (twiddle_spec foo_schema).
+ DECLARE _foo_twiddle  (twiddle_spec foo_invariant).
 
 Definition make_foo_spec :=
  DECLARE _make_foo
  WITH mtable: val
  PRE [ ]
     PROP () LOCAL (gvar _foo_methods mtable) 
-    SEP (object_methods foo_schema mtable)
+    SEP (object_methods foo_invariant mtable)
  POST [ tobject ]
     EX p: val, PROP () LOCAL (temp ret_temp p) 
-     SEP (object_mpred nil p; object_methods foo_schema mtable).
+     SEP (object_mpred nil p; object_methods foo_invariant mtable).
 
 Definition main_spec :=
  DECLARE _main
@@ -90,7 +87,7 @@ Definition Gprog : funspecs :=   ltac:(with_library prog [
 
 Lemma body_foo_reset: semax_body Vprog Gprog f_foo_reset foo_reset_spec.
 Proof.
-unfold foo_reset_spec, foo_schema, reset_spec.
+unfold foo_reset_spec, foo_invariant, reset_spec.
 start_function.
 simpl.
 Intros.
@@ -100,16 +97,17 @@ Qed.
 
 Lemma body_foo_twiddle: semax_body Vprog Gprog f_foo_twiddle foo_twiddle_spec.
 Proof.
-unfold foo_twiddle_spec, foo_schema, twiddle_spec.
+unfold foo_twiddle_spec, foo_invariant, twiddle_spec.
 start_function.
 simpl.
 Intros.
 forward.
 forward.
 forward.
+Exists (2 * fold_right Z.add 0 history + i).
+entailer!.
 replace (2 * (i + fold_right Z.add 0 history))%Z with (2* fold_right Z.add 0 history + 2 * i).
 entailer!.
-f_equal. f_equal. omega.
 omega.
 Qed.
 
@@ -128,16 +126,16 @@ apply pred_ext. apply andp_right; auto. apply andp_left2; auto.
 Qed.
 
 Lemma split_object_methods:
-  forall schema m, 
-    object_methods schema m |-- object_methods schema m * object_methods schema m.
+  forall instance m, 
+    object_methods instance m |-- object_methods instance m * object_methods instance m.
 Proof.
 intros.
 unfold object_methods.
 Intros sh reset twiddle.
 Exists (fst (Share.split sh)) reset twiddle.
 Exists (snd (Share.split sh)) reset twiddle.
-rewrite (split_func_ptr' (reset_spec schema) reset) at 1.
-rewrite (split_func_ptr' (twiddle_spec schema) twiddle) at 1.
+rewrite (split_func_ptr' (reset_spec instance) reset) at 1.
+rewrite (split_func_ptr' (twiddle_spec instance) twiddle) at 1.
 entailer!.
 split.
 apply slice.split_YES_ok1; auto.
@@ -163,7 +161,7 @@ Intros p.
    LOCAL (temp _p p; gvar _foo_methods mtable)
    SEP (malloc_token Tsh (sizeof (Tstruct _foo_object noattr)) p;
           memory_block Tsh (sizeof (Tstruct _foo_object noattr)) p;
-          object_methods foo_schema mtable)).
+          object_methods foo_invariant mtable)).
 change (Memory.EqDec_val p nullval) with (eq_dec p nullval).
 *
 if_tac; entailer.
@@ -188,9 +186,9 @@ forward.
 forward.
 Exists p.
 unfold object_mpred.
-Exists foo_schema mtable.
-sep_apply (split_object_methods foo_schema mtable).
-unfold object_invariant.
+Exists foo_invariant mtable.
+sep_apply (split_object_methods foo_invariant mtable).
+unfold foo_invariant.
 entailer!.
 simpl.
 unfold_field_at 1%nat.
@@ -213,8 +211,8 @@ ENTAIL Delta,
 PROP ( )
 LOCAL (gvar _foo_twiddle twiddle; gvar _foo_reset reset;
 gvar _foo_methods mtable)
-SEP (func_ptr' (reset_spec foo_schema) reset;
-      func_ptr' (twiddle_spec foo_schema) twiddle;
+SEP (func_ptr' (reset_spec foo_invariant) reset;
+      func_ptr' (twiddle_spec foo_invariant) twiddle;
      mapsto Ews
        (Tpointer
           (Tfunction
@@ -227,7 +225,7 @@ mapsto Ews
      (Tfunction (Tcons (Tpointer (Tstruct 1%positive noattr) noattr) Tnil)
         Tvoid cc_default) noattr) (offset_val 0 mtable) (offset_val 0 reset))
 |-- PROP ( )
-    LOCAL (gvar _foo_methods mtable)  SEP (object_methods foo_schema mtable).
+    LOCAL (gvar _foo_methods mtable)  SEP (object_methods foo_invariant mtable).
 Proof.
 intros.
 unfold object_methods.
@@ -283,44 +281,43 @@ Intros p.
 
 (* first method-call *)
 unfold object_mpred.
-Intros schema mtable0.
+Intros instance mtable0.
 forward.
 unfold object_methods at 1.
 Intros sh r0 t0.
 forward.
 forward_call (p, @nil Z).
 gather_SEP 1 2 3.
-replace_SEP 0 (object_methods schema mtable0).
+replace_SEP 0 (object_methods instance mtable0).
 unfold object_methods.
 entailer!. Exists sh r0 t0. entailer!.
 gather_SEP 0 1 2.
 replace_SEP 0 (object_mpred nil p).
-unfold object_mpred; entailer!. Exists schema mtable0; entailer!.
-drop_LOCALs [_p_reset; _mtable]. clear sh H r0 t0 mtable0 schema.
+unfold object_mpred; entailer!. Exists instance mtable0; entailer!.
+drop_LOCALs [_p_reset; _mtable]. clear sh H r0 t0 mtable0 instance.
 
 (* second method-call *)
 unfold object_mpred.
-Intros schema mtable0.
+Intros instance mtable0.
 forward.
 unfold object_methods at 1.
 Intros sh r0 t0.
 forward.
 forward_call (p, 3, @nil Z).
+computable.
+Intros i.
 gather_SEP 1 2 3.
-replace_SEP 0 (object_methods schema mtable0).
+replace_SEP 0 (object_methods instance mtable0).
 unfold object_methods.
 entailer!. Exists sh r0 t0. entailer!.
 gather_SEP 0 1 2.
 replace_SEP 0 (object_mpred [3] p).
-unfold object_mpred; entailer!. Exists schema mtable0; entailer!.
-drop_LOCALs [_p_twiddle; _mtable]. clear sh H r0 t0 mtable0 schema.
+unfold object_mpred; entailer!. Exists instance mtable0; entailer!.
+drop_LOCALs [_p_twiddle; _mtable]. clear sh H r0 t0 mtable0 instance.
 
 (* return *)
 forward.
 Qed.
-
-
-
 
 
 
